src/Examples/ExMach/RefinementAdequacy.v
@@ -1,0 +1,116 @@
+From iris.algebra Require Import auth gmap frac agree.
+Require Export CSL.WeakestPre CSL.Lifting CSL.Adequacy.
+Require Import Helpers.RelationTheorems.
+From iris.algebra Require Export functions.
+From iris.base_logic.lib Require Export invariants gen_heap.
+From iris.proofmode Require Export tactics.
+Require Export ExMach.ExMachAPI ExMach.WeakestPre.
+Require Export ExMach.SeqHeap.
+Set Default Proof Using "Type".
+
+Class exmachPreG Σ := ExMachPreG {
+  exm_preG_iris :> invPreG Σ;
+  exm_preG_mem :> seq_heapPreG nat nat Σ;
+  exm_preG_disk :> gen_heapPreG nat nat Σ
+}.
+
+Definition exmachΣ : gFunctors := #[invΣ; gen_heapΣ nat nat; seq_heapΣ nat nat].
+Instance subG_exmachPreG {Σ} : subG exmachΣ Σ → exmachPreG Σ.
+Proof. solve_inG. Qed.
+
+Import ExMach.
+
+(* We don't need to actually use this directly, because we're interested in showing refinements,
+   but worth proving first because it's a bit simpler and helps check that everything makes sense. *)
+Definition exmach_recovery_adequacy {T R} Σ `{exmachPreG Σ} s
+           (e: proc ExMach.Op T) (rec: proc _ R) σ φ φrec (φinv : forall {_ : exmachG Σ}, iProp Σ) :
+  state_wf σ →
+  (∀ `{exmachGenG Σ},
+      let H := exmachGen_set 0 in
+      (([∗ map] i ↦ v ∈ mem_state σ, i ↦ v @N)
+               ={⊤}=∗
+               WP e @ s; ⊤ {{ v, ⌜φ v⌝ }}
+               ∗ (|={⊤, ∅}=> φinv)
+               ∗ □ (∀ Hinv H0 H1 k,
+                      let H := @ExMachG Σ Hinv H0 H1 (S k) in
+                      (∃ Hinv, @φinv (@ExMachG Σ Hinv _ _ k))
+                      ={⊤}=∗ WP rec @ s; ⊤ {{ _, ⌜ φrec ⌝ }}
+                         ∗ (|={⊤, ∅}=>
+                         let _ := ExMachG Σ _ _ _ (exm_current) in φinv))
+      )%I) →
+  s = NotStuck →
+  @recv_adequate _ _ _ ExMach.l s e rec σ (λ v _, φ v) (λ _, φrec).
+Proof.
+  intros Hwf Hwp Hnot_stuck.
+  eapply (wp_recovery_adequacy _ _) with
+   (φinv0 := (fun s => ∃ _ : exmachG Σ, state_interp s ∗ φinv _)%I); auto.
+  iIntros (?) "".
+  iMod (seq_heap_strong_init
+          (fun i => if nat_eq_dec i 0 then mem_state σ else init_zero)) as (? Hpf_eq) "(Hmc&Hm)".
+  iMod (gen_heap_init (disk_state σ)) as (?) "Hd".
+  iExists (ex_mach_interp O).
+  iSplitL "Hmc Hd".
+  { simpl. iExists _, _. iFrame. iPureIntro.
+    destruct nat_eq_dec; last by congruence.
+    destruct Hwf as (Hwf1&Hwf2).
+    split_and!; eauto.
+    intros k ?.
+    destruct nat_eq_dec.
+    * lia.
+    * intuition.
+    * intros i. destruct (Hwf1 i). intuition.
+    * intros i. destruct (Hwf2 i). intuition.
+  }
+  iPoseProof (Hwp (ExMachGenG Σ _ _ _)) as "H".
+  iMod ("H" with "[Hm]") as "(Hwp&Hinv&#Hrec)"; iClear "H".
+  {
+    rewrite -Hpf_eq. iApply mem_init_to_bigOp0; auto.
+    destruct Hwf; auto.
+  }
+  iModIntro.
+  iSplitL "Hwp".
+  { iApply wp_wand_l; iFrame. iIntros.
+    iApply fupd_mask_weaken; first by set_solver+. auto. }
+  iSplitL "Hinv".
+  { iIntros.  iMod "Hinv". iModIntro. iExists _. iFrame; auto. }
+  iAlways. iIntros (invG ?? Hcrash) "Hinv".
+  iDestruct "Hinv" as (HexmachG) "(Hstate&Hinv)".
+  simpl in *.
+  iSpecialize ("Hrec" $! invG (@exm_mem_inG _ HexmachG) (@exm_disk_inG _ HexmachG)
+                      ((@exm_current Σ HexmachG)) with "[Hinv]").
+  { iExists (exm_invG). destruct HexmachG; auto. }
+  iMod "Hrec" as "(Hrec&Hinv)".
+  iModIntro.
+  iExists ((@ex_mach_interp Σ (@exm_disk_inG Σ HexmachG) (@exm_mem_inG Σ HexmachG)
+                            (S (@exm_current Σ HexmachG)))).
+  iSplitL "Hstate".
+  { (* shows ex_mach_interp is holds after crash for next gen *)
+    rewrite /ex_mach_interp.
+    iDestruct "Hstate" as (mems disks) "(?&?&%&Hp)".
+    iDestruct "Hp" as %(Hdisks&Hcrash'&Hwf1&Hwf2).
+    inversion Hcrash; subst.
+    iExists mems, _. iFrame.
+    iPureIntro. split_and!.
+    * eauto.
+    * rewrite /crash_fun//=.
+    * intros. eapply Hcrash'; eauto. lia.
+    * rewrite /crash_fun/=. intros i Hsome.
+      apply not_le; intros Hge.
+      rewrite init_zero_lookup_ge_None in Hsome; last by lia.
+      apply is_Some_None in Hsome; auto.
+    * rewrite /crash_fun; auto.
+  }
+  iSplitL "Hrec".
+  {
+    (* For some reason @wp_wand_l fails here, not sure why *)
+    iPoseProof (@wp_mono with "[Hrec]") as "H"; [| eauto |]; last eauto.
+    iIntros. iApply fupd_mask_weaken; auto.
+  }
+  iIntros.
+  iMod "Hinv". iModIntro.
+  iExists {| exm_invG := invG;
+             exm_mem_inG := HexmachG.(@exm_mem_inG Σ);
+             exm_disk_inG := HexmachG.(@exm_disk_inG Σ);
+             exm_current := S HexmachG.(@exm_current Σ) |}.
+  iFrame.
+Qed.
